coq/Common.v
@@ -11,7 +11,10 @@ Definition ClientId := nat.
 
 Definition Event: Set := Content.
 Definition Msg: Set := Content.
-Definition Packet: Set := ClientId * Msg.
+Record State : Set := mkPkt {
+  sender: ClientId;
+  msgof: Msg
+}.
 
 Definition update {T: Type} f (id: nat) (v: T) id' :=
   if Nat.eqb id id' then v
